add some proofs

S5/language.lean
@@ -1,16 +1,14 @@
 inductive form where 
   | atom : Nat → form 
-  | bot : form
+  | neg : form → form
   | impl : form → form → form 
   | box : form → form 
 
-set_option quotPrecheck false
-
-notation:40 "¬"p => form.impl p (form.bot)
+notation:40 "¬"p => form.neg p
 infix:50 "→" => form.impl 
 notation p "∧" q => ¬(p → (¬q))
 notation p "∨" q => ((¬p) ∧ (¬q))
 prefix:80 "□" => form.box 
 notation "⋄"p => ¬(□(¬p)) 
 notation "⊥" => form.bot
-notation "⊤" => ¬(form.bot)
+notation "⊤" => ¬⊥
